thys/LLL_Basis_Reduction/LLL_Complexity.thy
@@ -26,15 +26,13 @@ definition result :: "'a cost \<Rightarrow> 'a" where "result = fst"
 lemma cost_simps: "cost (a,c) = c" "result (a,c) = a" 
   unfolding cost_def result_def by auto
 
-context LLL
+context LLL_with_assms
 begin
 
 context
   fixes arith_cost :: nat
-  assumes \<alpha>: "\<alpha> > 4/3" and m0: "m \<noteq> 0" 
+  assumes \<alpha>_gt: "\<alpha> > 4/3" and m0: "m \<noteq> 0" 
 begin
-
-private lemma alpha: "\<alpha> \<ge> 4/3" using \<alpha> by auto
 
 fun basis_reduction_add_row_main_cost :: "state \<Rightarrow> int vec \<Rightarrow> rat \<Rightarrow> (state \<times> int) cost" where 
   "basis_reduction_add_row_main_cost (i,F,G) fj mu = (let     
@@ -149,7 +147,7 @@ definition basis_reduction_add_rows_cost :: "state \<Rightarrow> state cost" whe
         gjs = fst G
       in basis_reduction_add_row_i_all_main_cost state fjs gjs)" 
 
-lemma basis_reduction_add_rows_cost: assumes "LLL_invariant A state F G" 
+lemma basis_reduction_add_rows_cost: assumes "LLL_invariant state F G" 
   shows "result (basis_reduction_add_rows_cost state) = basis_reduction_add_rows state" (is ?g1)
      "cost (basis_reduction_add_rows_cost state) \<le> 4 * m * n * arith_cost" (is ?g2)
 proof -
@@ -173,7 +171,7 @@ definition basis_reduction_step_cost :: "state \<Rightarrow> state cost" where
 
 definition "body_cost = (4 * m + 12) * n * arith_cost" 
 
-lemma basis_reduction_step_cost: assumes "LLL_invariant A state F G" 
+lemma basis_reduction_step_cost: assumes "LLL_invariant state F G" 
   shows "result (basis_reduction_step_cost state) = basis_reduction_step \<alpha> state" (is ?g1)
      "cost (basis_reduction_step_cost state) \<le> body_cost" (is ?g2)
 proof -
@@ -195,7 +193,7 @@ qed
 function basis_reduction_main_cost :: "state \<Rightarrow> state cost" where
   "basis_reduction_main_cost state = (
      case state of (i,F,G) \<Rightarrow>
-     if i < m \<and> (\<exists> A FF GG. LLL_invariant A state FF GG) 
+     if i < m \<and> (\<exists> FF GG. LLL_invariant state FF GG) 
        \<comment> \<open>The check on the invariant is just to be able to prove termination. 
           One cannot use partial-function at this point, since the function with cost is not tail-recursive.\<close>
      then case basis_reduction_step_cost state of 
@@ -209,28 +207,28 @@ termination
 proof (standard, rule wf_measure[of LLL_measure], goal_cases)
   case (1 state i FG F G state1 c1)
   note * = 1(1)[symmetric] 1(2)[symmetric] 1(3) 1(4)[symmetric]
-  from * obtain FF GG A where i: "i < m" and inv: "LLL_invariant A (i, F, G) FF GG" by auto
+  from * obtain FF GG where i: "i < m" and inv: "LLL_invariant (i, F, G) FF GG" by auto
   from basis_reduction_step_cost[OF inv, unfolded *] 
   have res: "basis_reduction_step \<alpha> (i, F, G) = state1" using * cost_simps(2) by metis
-  from basis_reduction_step[OF alpha inv i res]
+  from basis_reduction_step[OF inv i res]
   show ?case unfolding * by auto
 qed
 
 declare basis_reduction_main_cost.simps[simp del]
 
-definition "num_loops A = m + 2 * m * m * nat (ceiling (log (4 * of_rat \<alpha> / (4 + of_rat \<alpha>)) (real A)))"
+definition "num_loops = m + 2 * m * m * nat (ceiling (log base (real A)))"
 
-lemma basis_reduction_main_cost: fixes F G assumes "LLL_invariant A state F G"
+lemma basis_reduction_main_cost: fixes F G assumes "LLL_invariant state F G"
   shows "result (basis_reduction_main_cost state) = basis_reduction_main \<alpha> m state" (is ?g1) 
-   "cost (basis_reduction_main_cost state) \<le> body_cost * num_loops A" (is ?g2)
+   "cost (basis_reduction_main_cost state) \<le> body_cost * num_loops" (is ?g2)
 proof -
-  have inv: "LLL_partial_invariant A state F G" using assms unfolding LLL_invariant_def by auto
+  have inv: "LLL_partial_invariant state F G" using assms unfolding LLL_invariant_def by auto
   have ?g1 and cost: "cost (basis_reduction_main_cost state) \<le> body_cost * LLL_measure state"
     using assms
   proof (atomize (full), induct state arbitrary: F G rule: wf_induct[OF wf_measure[of LLL_measure]])
     case (1 state F G)
     note inv = 1(2)
-    have ex: "(\<exists>A FF. Ex (LLL_invariant A state FF)) = True" using inv by auto
+    have ex: "(\<exists>FF. Ex (LLL_invariant state FF)) = True" using inv by auto
     note IH = 1(1)[rule_format]
     obtain i Fr1 Gr1 where state: "state = (i,Fr1,Gr1)" by (cases state, auto)
     note inv = inv[unfolded state]
@@ -247,8 +245,8 @@ proof -
         by (cases ?rec, auto)
       note simp = simp[unfolded rec split]
       from simp i have res: "basis_reduction_main_cost state = (state2, c1 + c2)" by auto    
-      note bsr = basis_reduction_step[OF alpha inv i bb]
-      from bsr(1) obtain F' G' where inv: "LLL_invariant A state1 F' G'" by auto
+      note bsr = basis_reduction_step[OF inv i bb]
+      from bsr(1) obtain F' G' where inv: "LLL_invariant state1 F' G'" by auto
       from bsr(2) have "(state1 ,state) \<in> measure LLL_measure" by (auto simp: state)
       from IH[OF this inv, unfolded rec cost_simps]
       have res': "basis_reduction_main \<alpha> m state1 = state2" 
@@ -267,15 +265,15 @@ proof -
   qed
   show ?g1 by fact
   obtain i F G where state: "state = (i, F, G)" by (cases state, auto)
-  note cost also have "body_cost * LLL_measure state \<le> body_cost * num_loops A" 
+  note cost also have "body_cost * LLL_measure state \<le> body_cost * num_loops" 
   proof (rule mult_left_mono; linarith?)
-    define l where "l = log (4 * real_of_rat \<alpha> / (4 + real_of_rat \<alpha>)) (real A)" 
+    define l where "l = log base (real A)" 
     define k where "k = 2 * m * m" 
     have "LLL_measure state \<le> nat (ceiling (m + k * l))" unfolding l_def k_def
-      using LLL_measure_approx[OF alpha inv[unfolded state] \<alpha> m0, folded state] by linarith
-    also have "\<dots> \<le> num_loops A" unfolding num_loops_def l_def[symmetric] k_def[symmetric]
+      using LLL_measure_approx[OF inv[unfolded state] \<alpha>_gt m0, folded state] by linarith
+    also have "\<dots> \<le> num_loops" unfolding num_loops_def l_def[symmetric] k_def[symmetric]
       by (simp add: of_nat_ceiling times_right_mono)
-    finally show "LLL_measure state \<le> num_loops A" .
+    finally show "LLL_measure state \<le> num_loops" .
   qed
   finally show ?g2 . 
 qed
@@ -375,19 +373,10 @@ definition reduce_basis_cost :: "int vec list \<Rightarrow> int vec list cost" w
   "reduce_basis_cost F = (case basis_reduction_state_cost F of (state,c) \<Rightarrow> 
     ((of_list_repr o fst o snd) state, c))" 
 
-definition "max_sqnorm (F :: int vec list) = max_list (map (nat o sq_norm) F)" 
-
-context
-  fixes F :: "int vec list" 
-  assumes len: "length F = m"
-  and lin_dep: "gs.lin_indpt_list (RAT F)" 
-  and L: "lattice_of F = L" 
-begin
-
-lemma initial_state_cost: "result (initial_state_cost F) = initial_state n F" (is ?g1)
-  "cost (initial_state_cost F) \<le> initial_gso_cost" (is ?g2)
+lemma initial_state_cost: "result (initial_state_cost fs_init) = initial_state n fs_init" (is ?g1)
+  "cost (initial_state_cost fs_init) \<le> initial_gso_cost" (is ?g2)
 proof -
-  let ?F = "map (map_vec rat_of_int) F" 
+  let ?F = "map (map_vec rat_of_int) fs_init" 
   have len: "length ?F \<le> m" using len by auto
   obtain G c where gso: "gram_schmidt_triv_cost ?F = (G,c)" (is "?gso = _")
     by (cases ?gso, auto)
@@ -397,21 +386,21 @@ proof -
 qed
 
 lemma basis_reduction_state_cost: 
-   "result (basis_reduction_state_cost F) = basis_reduction_state n \<alpha> F"  (is ?g1)
-   "cost (basis_reduction_state_cost F) \<le> initial_gso_cost + body_cost * num_loops (max_sqnorm F)" (is ?g2)
+   "result (basis_reduction_state_cost fs_init) = basis_reduction_state n \<alpha> fs_init"  (is ?g1)
+   "cost (basis_reduction_state_cost fs_init) \<le> initial_gso_cost + body_cost * num_loops" (is ?g2)
 proof -
-  obtain state1 c1 where init: "initial_state_cost F = (state1, c1)" (is "?init = _") by (cases ?init, auto)
+  obtain state1 c1 where init: "initial_state_cost fs_init = (state1, c1)" (is "?init = _") by (cases ?init, auto)
   obtain state2 c2 where main: "basis_reduction_main_cost state1 = (state2, c2)" (is "?main = _") by (cases ?main, auto)
-  have res: "basis_reduction_state_cost F = (state2, c1 + c2)" 
+  have res: "basis_reduction_state_cost fs_init = (state2, c1 + c2)" 
     unfolding basis_reduction_state_cost_def init main split by simp
   from initial_state_cost[unfolded init cost_simps]
-  have c1: "c1 \<le> initial_gso_cost" and init: "initial_state n F = state1" by auto
-  from initial_state[OF alpha lin_dep len L init refl, folded max_sqnorm_def]
-  obtain F' G' where inv: "LLL_invariant (max_sqnorm F) state1 F' G'" by auto
+  have c1: "c1 \<le> initial_gso_cost" and init: "initial_state n fs_init = state1" by auto
+  from initial_state[OF init]
+  obtain F' G' where inv: "LLL_invariant state1 F' G'" by auto
   from basis_reduction_main_cost[OF inv, unfolded main cost_simps]
-  have main: "basis_reduction_main \<alpha> m state1 = state2" and c2: "c2 \<le> body_cost * num_loops (max_sqnorm F)" 
+  have main: "basis_reduction_main \<alpha> m state1 = state2" and c2: "c2 \<le> body_cost * num_loops" 
     by auto
-  have res': "basis_reduction_state n \<alpha> F = state2" unfolding basis_reduction_state_def len init main ..
+  have res': "basis_reduction_state n \<alpha> fs_init = state2" unfolding basis_reduction_state_def len init main ..
   show ?g1 unfolding res res' cost_simps ..
   show ?g2 unfolding res cost_simps using c1 c2 by auto
 qed
@@ -422,30 +411,25 @@ text \<open>The lemma for the LLL algorithm with explicit cost annotations @{con
   the same as in the non-cost counting @{const reduce_basis}.\<close>
 
 lemma reduce_basis_cost: 
-   "result (reduce_basis_cost F) = fst (reduce_basis n \<alpha> F)"  (is ?g1)
-   "cost (reduce_basis_cost F) \<le> initial_gso_cost + body_cost * num_loops (max_sqnorm F)" (is ?g2)
+   "result (reduce_basis_cost fs_init) = fst (reduce_basis n \<alpha> fs_init)"  (is ?g1)
+   "cost (reduce_basis_cost fs_init) \<le> initial_gso_cost + body_cost * num_loops" (is ?g2)
 proof -
-  obtain state c where b: "basis_reduction_state_cost F = (state,c)" (is "?b = _") by (cases ?b, auto)
+  obtain state c where b: "basis_reduction_state_cost fs_init = (state,c)" (is "?b = _") by (cases ?b, auto)
   from basis_reduction_state_cost[unfolded b cost_simps]
-  have bb: "basis_reduction_state n \<alpha> F = state" and c: "c \<le> initial_gso_cost + body_cost * num_loops (max_sqnorm F)" 
+  have bb: "basis_reduction_state n \<alpha> fs_init = state" and c: "c \<le> initial_gso_cost + body_cost * num_loops" 
     by auto
   show ?g1 ?g2 unfolding reduce_basis_cost_def reduce_basis_def b bb split cost_simps fst_conv using c by auto
 qed
 
 text \<open>Theorem with expanded costs: $O(n\cdot m^3 \cdot \log (\mathit{maxnorm}\ F))$ arithmetic operations\<close>
 lemma reduce_basis_cost_expanded: 
-  assumes "A = max_list (map (nat \<circ> sq_norm) F)" 
-  and "Log = nat \<lceil>log (4 * of_rat \<alpha> / (4 + of_rat \<alpha>)) A\<rceil>" 
-  shows "cost (reduce_basis_cost F)
+  assumes "Log = nat \<lceil>log (of_rat (4 * \<alpha> / (4 + \<alpha>))) AA\<rceil>"   
+  and "AA = max_list (map (nat \<circ> sq_norm) fs_init)" 
+  shows "cost (reduce_basis_cost fs_init)
   \<le> (4 * m * m + 3 * m + (4 * m * m + 12 * m) * (1 + 2 * m * Log)) * n * arith_cost"
-  unfolding assms
-  using reduce_basis_cost(2)[unfolded num_loops_def max_sqnorm_def body_cost_def initial_gso_cost_def]
+  unfolding assms A_def[symmetric]
+  using reduce_basis_cost(2)[unfolded num_loops_def body_cost_def initial_gso_cost_def base_def]
   by (auto simp: nat_distrib ac_simps)
-
-end (* lin-indep F *)
 end (* fixing arith_cost and assume \<alpha> > 4/3 *)
-end (* LLL locale which fixes n m \<alpha> L *)
-
-text \<open>Expanded theorem outside locale listing all preconditions\<close>
-thm LLL.reduce_basis_cost_expanded[OF _ _ refl _ refl]
+end (* LLL locale *)
 end (* theory *)
